various changes

bin/lxr_controller.ml
@@ -1,6 +1,6 @@
 open Lwt
 
-open Elykseer__Lxr
+(* open Elykseer__Lxr *)
 open Elykseer__Lxr.Environment
 
 open Elykseer_utils
@@ -24,22 +24,25 @@ let anon_args_fun _fn = ()
         Lwt_list.iter_s (fun fb -> Lwt_io.printl(Utils.fibs2s fb)) fbs
     ) abs *)
 
-let run abs =
-    if !arg_verbose
-    then List.map (fun (anum,fbs) -> print_string("anum = "); print_int(Conversion.p2i anum); print_endline("");
-             List.map (fun fb -> print_endline @@ Utils.fibs2s fb) fbs
-         ) abs |> ignore
+let run es =
+    (* if !arg_verbose
+    then List.map (fun e -> print_endline @@ Utils.e2s e) es |> ignore
     else ()
-    ;
+    ; *)
     let pool = Lwt_pool.create !arg_nproc
-                  ~dispose: (fun p -> if !arg_verbose then print_endline("dispose process.") else ();
+                  ~validate: (fun _ -> Lwt.return false) (* force the creation of new processes *)
+                  ~dispose: (fun p -> (if !arg_verbose then Lwt_io.printf "dispose process." else Lwt.return ()) |> ignore;
                                       p#close >|= ignore)
                   (fun () ->
                       if !arg_verbose then print_endline("starting process.") else ();
-                      Lwt_process.open_process("", [|"echo"; "calling lxr_encoder"|]) |> Lwt.return) in
+                      Lwt_process.open_process("", [|"sleep"; "5" |]) |> Lwt.return) in
     
-    let processor i (_idx,fibs) p =
-      (if !arg_verbose then Lwt_io.printf "  process %d:\n  assembly: %s\n" i (String.concat "; " (List.map Utils.fibs2s fibs)) else Lwt.return ()) |> ignore;
+    let processor i e p =
+      (if !arg_verbose
+       then Lwt_io.printf "  process %d:\n%s\n" i (Utils.e2j e)
+       else Lwt.return ()) |> ignore;
+      let%lwt () = Lwt_io.write_line p#stdin (Utils.e2j e) in
+      let%lwt () = Lwt_io.flush p#stdin in
       Lwt_io.read_lines p#stdout |>
       Lwt_stream.iter_s Lwt_io.printl in
     
@@ -48,16 +51,17 @@ let run abs =
         if k <= 0 then l else loop (k - 1) (k :: l) in
       loop n [] in
 
-    mklist (List.length abs) |>
+    mklist (List.length es) |>
       Lwt_stream.of_list |>
-      Lwt_stream.iter_p (fun i -> Lwt_pool.use pool (processor i (List.nth abs (i - 1))))
+      Lwt_stream.iter_p (fun i -> Lwt_pool.use pool (processor i (List.nth es (i - 1))))
 
 (* main *)
 let main () = Arg.parse argspec anon_args_fun "lxr_controller: vfj";
     let _setup = setup_environment in
     let e = Envutils.envrestore !arg_fctrl in
-    let abs = Envutils.env2assemblies e in
-    (* lwt_print abs *)
-    run abs
+    let es = Envutils.env2assemblies e in
+    let res = run es in
+    Unix.sleep 3;
+    res
 
 let () = Lwt_main.run (main ())
