bin/lxr_encoder.ml
@@ -1,6 +1,8 @@
 (* open Lwt *)
 
-(* open Elykseer__Lxr *)
+open Elykseer__Lxr
+open Elykseer__Lxr.Assembly
+open Elykseer__Lxr.Block
 open Elykseer__Lxr.Environment
 
 open Elykseer_utils
@@ -16,11 +18,109 @@ let argspec =
 
 let anon_args_fun _fn = ()
 
+(* let mklist n dec =
+  let rec loop k l =
+    if k <= 0 then l else loop (k - dec) (k :: l) in
+  loop n [] *)
+
+(* the block size *)
+(* let blocksize = ref 2048;; *)
+
+
+(* let read_file_block _ch _buf _apos bsz =
+    if bsz <= 0 then Lwt.return 0
+    else
+      (* Lwt_io.read_into_bigstring ch !buf apos 2024 *)
+      (* Lwt_io.read_into ch buf apos 2024 *)
+      Lwt.return (min bsz 2024) *)
+
+(* let read_file_blocks ch buf apos0 bsz0 bn0 fpos0 banum =
+    let apos = ref apos0 in
+    let bsz = ref bsz0 in
+    let bn = ref bn0 in
+    let fpos = ref fpos0 in
+    Lwt_stream.fold_s (fun i agg ->
+        let%lwt () = Lwt_io.printf "@%d: reading from %d len=%d into pos=%d\n" i !fpos !bsz !apos in
+        match%lwt read_file_block ch buf !apos !bsz with
+        | 0 -> Lwt.return agg
+        | n -> let%lwt () = Lwt_io.printf "read %d\n\n" n in
+               let bs = { blockid = Conversion.i2p !bn
+                        ; blocksize = Conversion.i2n n
+                        ; filepos = Conversion.i2n !fpos
+                        ; blockanum = banum
+                        ; blockapos = Conversion.i2n !apos } :: agg in
+               apos := !apos + n;
+               bsz := !bsz - n;
+               bn := !bn + 1;
+               fpos := !fpos + n;
+               Lwt.return bs )
+        (Lwt_stream.of_list @@ mklist !bsz !blocksize)
+        [] *)
+
+(* let read_file_blocks _ch _buf apos _bsz0 bn fpos banum =
+    let bi = { blockid = Conversion.i2p bn
+             ; bchecksum = ""
+             ; blocksize = Conversion.i2n 42
+             ; filepos = Conversion.i2n fpos
+             ; blockanum = banum
+             ; blockapos = Conversion.i2n apos } in
+    Lwt.return [bi] *)
+
+let encode_file fb _buf : fileblocks Lwt.t =
+    let%lwt () = Lwt_io.printl (Utils.fibs2s fb) in
+    let%lwt _bs = Lwt_io.with_file ~mode:Input fb.bfi.fname
+      (fun _ch ->
+        Lwt_stream.fold_s (fun b _agg ->
+            (* fseek ch b.filepos *)
+            let _fpos = (Conversion.n2i b.filepos) in
+            let _bsz = (Conversion.n2i b.blocksize) in
+            (* let%lwt () = Lwt_io.set_position ch @@ Int64.of_int fpos in *)
+            (* let fbytes = fread ch b.blocksize in *)
+            (* let%lwt bs = read_file_blocks ch buf (Conversion.n2i b.blockapos) bsz
+                                                  0 fpos b.blockanum  in *)
+            (* let n = List.fold_left (fun agg b -> agg + Conversion.n2i b.blocksize) 0 bs in *)
+            (* let%lwt () = Lwt_io.printf "read %d bytes of %d\n" n bsz in *)
+            (* add_to_buf buf b.blockapos fbytes *)
+            (* Lwt.return (bs @ agg) ) *)
+            Lwt.return [] )
+            (Lwt_stream.of_list fb.blocks)
+            []
+      ) in
+    Lwt.return fb 
+    (* { bfi = fb.bfi; blocks = bs } *)
+
+let encode e : fileblocks list Lwt.t =
+    let len =   (Conversion.n2i chunkwidth_N)
+              * (Conversion.n2i chunklength_N)
+              * (Conversion.p2i (nchunks (List.hd e.assemblies))) in
+    let%lwt () = Lwt_io.printf "assembly size %d bytes\n" len in
+    (* let buf = ref (Lwt_bytes.create len) in *)
+    (* let buf = Bytes.create len in *)
+    let buf = [0] in
+    Lwt_stream.fold_s (fun fb agg -> let%lwt fb' = encode_file fb buf in
+                                     Lwt.return (fb' :: agg))
+                      (Lwt_stream.of_list e.files)
+                      []
+
+let encode_check e : environment Lwt.t =
+    if List.length e.assemblies = 1
+    then let%lwt fs = encode e in
+         let%lwt () = Lwt_io.printf "encoded %d files" (List.length fs) in
+         (* Lwt.return e *)
+         let cnt = List.fold_left (fun agg f -> agg + List.fold_left (fun agg b -> agg + Conversion.n2i b.blocksize) 0 f.blocks) 0 e.files in
+         Lwt.return { cur_assembly = e.cur_assembly
+                    ; count_input_bytes = Conversion.i2n cnt
+                    ; config = e.config
+                    ; files = fs
+                    ; assemblies = e.assemblies }
+    else Lwt.return e
 
 (* main *)
 let main () = Arg.parse argspec anon_args_fun "lxr_encoder: vf";
     let _setup = setup_environment in
     let e = Envutils.envrestore !arg_fctrl in
-    Lwt_io.printl (Utils.e2s e)
+    let%lwt () = Lwt_io.printl (Utils.e2s e) in
+    let%lwt e' = encode_check e in
+    Lwt_io.printf "encoded %d bytes\n" @@ Conversion.n2i(e'.count_input_bytes)
 
 let () = Lwt_main.run (main ())
