elykseer-utils/envutils.mli
@@ -1,5 +1,5 @@
 
-open Elykseer__Lxr
+(* open Elykseer__Lxr *)
 open Elykseer__Lxr.Configuration
 open Elykseer__Lxr.Environment
 
@@ -7,4 +7,4 @@ val envload : configuration -> string -> environment
 
 val envrestore : string -> environment
 
-val env2assemblies : environment -> (positive * Block.fileblocks list) list
+val env2assemblies : environment -> environment list
