theories/Block.v
@@ -6,7 +6,7 @@ Module Export Block.
 
 Require Import NArith.
 From Coq Require Import NArith.BinNat.
-(* From Coq Require Import Strings.String Strings.Byte. *)
+From Coq Require Import Strings.String.
 
 Open Scope N_scope.
 
@@ -16,6 +16,7 @@ From LXR Require Import Filetypes.
 Record blockinformation : Type :=
     mkblockinformation
         { blockid : positive
+        ; bchecksum : string
         ; blocksize : N
         ; filepos : N
         ; blockanum : positive
@@ -25,6 +26,7 @@ Record blockinformation : Type :=
 Record fileblocks : Type :=
     mkfileblocks
         { bfi : fileinformation
+        ; fversion : positive
         ; blocks : list blockinformation
         }.
 
