theories/Buffer.v
@@ -16,19 +16,20 @@ Unset Printing Implicit Defensive.
 
 From Coq Require Import Lia.
 Require Import ZArith NArith.
-Open Scope positive_scope.
+(* Open Scope positive_scope. *)
+Open Scope N_scope.
 
 Record buffer : Type := mkbuffer
-    { width : positive
-    ; height : positive
+    { width : N
+    ; height : N
     }.
-Definition new_buffer (w h : positive) : buffer :=
+Definition new_buffer (w h : N) : buffer :=
     {| width := w; height := h |}.
 
-Definition set (b : buffer) (idx : positive) (v : positive) : Prop :=
+Definition set (b : buffer) (idx : N) (v : Z) : Prop :=
     idx < (width b) * (height b).
 
-Definition get (b : buffer) (idx : positive) : Prop :=
+Definition get (b : buffer) (idx : N) : Prop :=
     idx < (width b) * (height b).
 
 End Buffer.
