theories/Example.v
@@ -38,22 +38,23 @@ Lemma test1 :
     let setup := setup_environment in
     let e := initial_environment config0 in
     let fi := fi_t1_dat in
-    let bi := {| blockid := 1; blocksize := 4194304; filepos := 0; blockanum := 1; blockapos := 0 |} in
+    let bi := {| blockid := 1; blocksize := 4194304; bchecksum := "1";
+                 filepos := 0; blockanum := 1; blockapos := 0 |} in
     backup_file config0 e "t1.dat" =
     {| cur_assembly := {|
                         nchunks := 16;
                         anum := 2; aid := Utilities.Utilities.rnd256 11111;
-                        valid := valid_assembly_size 16;
+                        (* valid := valid_assembly_size 16; *)
                         apos := 0; (*N.min (assemblysz config0) 33;*)
                         encrypted := false;
-                        (* chunks := mk_chunk_list 16 1 *)
+                        chunks := mk_chunk_list 16 2
                        |} 
     ;  count_input_bytes := 4194304
     ;  config := {| num_chunks := 16; path_chunks := "./lxr"; path_meta := "./meta"; my_id := 11111 |}
-    ;  files := {| bfi:= fi;
+    ;  files := {| bfi:= fi; fversion := 1;
                    blocks := bi :: nil |} :: nil
-    ;  assemblies := {| nchunks := 16; anum := 2; aid := Utilities.Utilities.rnd256 11111; valid := valid_assembly_size 16; apos := 0; encrypted := false; |} ::
-                     {| nchunks := 16; anum := 1; aid := Utilities.Utilities.rnd256 11111; valid := valid_assembly_size 16; apos := 4194304; encrypted := false; |} :: nil
+    ;  assemblies := {| nchunks := 16; anum := 2; aid := Utilities.Utilities.rnd256 11111; (* valid := valid_assembly_size 16; *) apos := 0; encrypted := false; chunks := mk_chunk_list 16 2 |} ::
+                     {| nchunks := 16; anum := 1; aid := Utilities.Utilities.rnd256 11111; (* valid := valid_assembly_size 16; *) apos := 4194304; encrypted := false; chunks := mk_chunk_list 16 1 |} :: nil
     |}.
 Proof. intros.
     unfold backup_file.
@@ -70,26 +71,28 @@ Example fi_t2_dat : fileinformation := {| fname := "t2.dat"; fsize := 1048576; f
 Lemma test2 :
     let e0 := initial_environment config0 in
     let fi1 := fi_t1_dat in
-    let bi1 := {| blockid := 1; blocksize := 4194304; filepos := 0; blockanum := 1; blockapos := 0 |} in
+    let bi1 := {| blockid := 1; blocksize := 4194304; bchecksum := "1";
+                  filepos := 0; blockanum := 1; blockapos := 0 |} in
     let e1 := backup_file' config0 e0 fi1 in
     let fi2 := fi_t2_dat in
     backup_file config0 e1 "t2.dat" =
     {| cur_assembly := {|
                         nchunks := 16;
                         anum := 2; aid := Utilities.Utilities.rnd256 11111;
-                        valid := valid_assembly_size 16;
+                        (* valid := valid_assembly_size 16; *)
                         apos := 1048576;
                         encrypted := false;
-                        (* chunks := mk_chunk_list 16 1 *)
+                        chunks := mk_chunk_list 16 2
                        |} 
     ;  count_input_bytes := 4194304 + 1048576
     ;  config := {| num_chunks := 16; path_chunks := "./lxr"; path_meta := "./meta"; my_id := 11111 |}
-    ;  files := {| bfi:= fi_t2_dat
-                  ; blocks := {| blockid := 1; blocksize := 1048576; filepos := 0; blockanum := 2; blockapos := 0 |} :: nil |}
-                ::  {| bfi := fi1
+    ;  files := {| bfi:= fi_t2_dat; fversion := 1
+                 ; blocks := {| blockid := 1; blocksize := 1048576; bchecksum := "1"
+                              ; filepos := 0; blockanum := 2; blockapos := 0 |} :: nil |}
+                ::  {| bfi := fi1; fversion := 1
                      ; blocks := bi1 :: nil |} :: nil
-    ;  assemblies := {| nchunks := 16; anum := 2; aid := Utilities.Utilities.rnd256 11111; valid := valid_assembly_size 16; apos := 1048576; encrypted := false; |} ::
-                     {| nchunks := 16; anum := 1; aid := Utilities.Utilities.rnd256 11111; valid := valid_assembly_size 16; apos := 4194304; encrypted := false; |} :: nil
+    ;  assemblies := {| nchunks := 16; anum := 2; aid := Utilities.Utilities.rnd256 11111; (* valid := valid_assembly_size 16; *) apos := 1048576; encrypted := false; chunks := mk_chunk_list 16 2 |} ::
+                     {| nchunks := 16; anum := 1; aid := Utilities.Utilities.rnd256 11111; (* valid := valid_assembly_size 16; *) apos := 4194304; encrypted := false; chunks := mk_chunk_list 16 1 |} :: nil
     |}.
 Proof. intros.
     vm_compute (backup_file' config0 e0 fi1) in * |-.
